Fuuuuck

week_39b_arithmetic_expressions.v
@@ -19,7 +19,8 @@ Notation "A =n= B" := (beq_nat A B) (at level 70, right associativity).
 Inductive arithmetic_expression : Type :=
   | Lit : nat -> arithmetic_expression
   | Plus : arithmetic_expression -> arithmetic_expression -> arithmetic_expression
-  | Times : arithmetic_expression -> arithmetic_expression -> arithmetic_expression.
+  | Times : arithmetic_expression -> arithmetic_expression -> arithmetic_expression
+  | Minus : arithmetic_expression -> arithmetic_expression -> arithmetic_expression.
 
 (* Exercise 0:
    Write samples of arithmetic expressions.
@@ -41,13 +42,14 @@ Definition specification_of_interpret (interpret : arithmetic_expression -> nat)
      interpret (Plus ae1 ae2) = (interpret ae1) + (interpret ae2))
   /\
   (forall ae1 ae2 : arithmetic_expression,
-     interpret (Times ae1 ae2) = (interpret ae1) * (interpret ae2)).
+     interpret (Times ae1 ae2) = (interpret ae1) * (interpret ae2))
+  /\
+  (forall ae1 ae2 : arithmetic_expression,
+     interpret (Minus ae1 ae2) = (interpret ae1) - (interpret ae2)).
 
 (* Exercise 1:
    Write unit tests.
 *)
-
-
 
 (* TODO: Lav nogle flere *)
 Definition unit_test_for_interpret (interpret : arithmetic_expression -> nat) :=
@@ -58,6 +60,7 @@ Definition unit_test_for_interpret (interpret : arithmetic_expression -> nat) :=
   (interpret (Plus (Lit 1) (Plus (Lit 2) (Lit 3))) =n= 6)
   &&
   (interpret (Times (Plus (Lit 1) (Lit 2)) (Plus (Lit 2) (Lit 3))) =n= 15)
+  && (interpret (Times (Times (Lit 2) (Lit 3)) (Times (Lit 4) (Lit 5))) =n= 120)
   .
 
 (* Exercise 2:
@@ -71,10 +74,64 @@ Fixpoint interpreter ( ae : arithmetic_expression) : nat :=
     | Lit n => n
     | Plus ae1 ae2 => (interpreter ae1) + (interpreter ae2)
     | Times ae1 ae2 => (interpreter ae1) * (interpreter ae2)
+    | Minus ae1 ae2 => (interpreter ae1) - (interpreter ae2)
   end.
 
 Compute (interpreter (Times (Lit 7) (Plus (Lit 5) (Lit 6)))).
 Compute unit_test_for_interpret interpreter.
+
+Lemma unfold_interpreter_lit :
+  forall n : nat,
+    interpreter (Lit n) = n.
+Proof.
+  unfold_tactic interpreter.
+Qed.
+
+Lemma unfold_interpreter_times :
+  forall a b : arithmetic_expression,
+    interpreter (Times a b) = (interpreter a) * (interpreter b).
+Proof.
+  unfold_tactic interpreter.
+Qed.
+
+Lemma unfold_interpreter_plus : 
+  forall a b : arithmetic_expression,
+    interpreter (Plus a b) = (interpreter a) + (interpreter b).
+Proof.
+  unfold_tactic interpreter.
+Qed.
+
+Lemma unfold_interpreter_minus :
+  forall a b : arithmetic_expression,
+    interpreter (Minus a b) = (interpreter a) - (interpreter b).
+Proof.
+  unfold_tactic interpreter.
+Qed.
+
+  
+Lemma interpreter_fits_the_specification_of_interpreter :
+  forall exp : arithmetic_expression,
+    specification_of_interpret interpreter.
+Proof.
+  unfold specification_of_interpret.
+  split.
+    
+    intro n.
+    apply (unfold_interpreter_lit n).
+
+    split.
+
+      intros ae1 ae2.
+      apply (unfold_interpreter_plus ae1 ae2).
+      
+      split.
+        intros ae1 ae2.
+        apply (unfold_interpreter_times ae1 ae2).
+
+        intros ae1 ae2.
+        apply (unfold_interpreter_minus ae1 ae2).
+
+Qed.
 
 
 (* Byte-code instructions: *)
@@ -82,7 +139,8 @@ Compute unit_test_for_interpret interpreter.
 Inductive byte_code_instruction : Type :=
   | PUSH : nat -> byte_code_instruction
   | ADD : byte_code_instruction
-  | MUL : byte_code_instruction.
+  | MUL : byte_code_instruction
+  | SUB : byte_code_instruction.
 
 (* ********** *)
 
@@ -113,12 +171,12 @@ Definition data_stack := list nat.
    For now, if the stack underflows, just assume it contains zeroes.
 *)
 
-Compute( 1 :: 2 :: 3 :: nil).
-Compute( head ( 1 :: 2 :: 3 :: nil)).
 
 (*
   Also, execute_byte_code_instruction is not recursive, so make sure to define it with Definition, not with Fixpoint.
 *)
+
+(* TODO: Skal vi ændre den måde x :: stack virker? *)
 Definition execute_byte_code_instruction (instruction : byte_code_instruction) ( dstack : data_stack) : data_stack :=
   match instruction with
     | PUSH n => n :: dstack
@@ -127,16 +185,24 @@ Definition execute_byte_code_instruction (instruction : byte_code_instruction) (
                | x :: stack => x :: stack
                | nil => 0 :: nil                                    
              end
-    | MIL => match dstack with
+    | MUL => match dstack with
                | x :: y :: stack => (mult x y) :: stack
                | x :: stack => x :: stack
                | nil => 0 :: nil
              end                                 
+    | SUB => match dstack with
+               | x :: y :: stack => (minus x y) :: stack
+               | x :: stack => x :: stack
+               | nil => 0 :: nil
+             end                                             
   end. 
+
 
 Compute(execute_byte_code_instruction (PUSH 4) (1 :: 2 :: nil)).
 Compute(execute_byte_code_instruction (MUL) (nil)).
 Compute(execute_byte_code_instruction (MUL) (3 :: 2 :: nil)).
+Compute(execute_byte_code_instruction (MUL) (1 :: nil)).
+
 
 
 (* ********** *)
@@ -168,17 +234,6 @@ Compute(execute_byte_code_program ((PUSH 4) :: (PUSH 3) :: (MUL) :: nil) (0 :: n
   DOING INDUCTION ON P1
 *)
 
-Lemma plus_plus : 
-  forall p : byte_code_program,
-    nil ++ p = p.
-Proof.
-  intro p.
-  (* C-c C-a C-n  _ ++ _*)
-  unfold app.
-  reflexivity.
-Qed.
-
-
 Lemma unfold_byte_code_program_bc : 
   forall s : data_stack,
     execute_byte_code_program nil s = s.
@@ -194,26 +249,27 @@ Proof.
   unfold_tactic execute_byte_code_program.
 Qed.
 
-Theorem list_of_programs : 
+Theorem about_list_of_instructions : 
   forall ( p1 p2 : byte_code_program) (s : data_stack),
-    execute_byte_code_program p1 (execute_byte_code_program p2 s) =
+    execute_byte_code_program p2 (execute_byte_code_program p1 s) =
     execute_byte_code_program  (p1 ++ p2) s.
 Proof.         
   intros p1 p2.
-  intro s.
+  induction p1 as [ | p1' p1s' IHsp1'].
 
-  induction p1 as [ | p1' IHp1' IHsp1'].
-  rewrite -> plus_plus.
+  intro s.
+  unfold app.
   rewrite -> unfold_byte_code_program_bc.
   reflexivity.
 
+  intro s.
   rewrite -> unfold_byte_code_program_ic.
+  rewrite <- (app_comm_cons).
+  rewrite -> (unfold_byte_code_program_ic).
+  rewrite -> (IHsp1' (execute_byte_code_instruction p1' s)).
+  reflexivity.
+Qed.
   
-Admitted.
-  
-
-
-
 
 (* ********** *)
 
@@ -222,10 +278,13 @@ Definition specification_of_compile (compile : arithmetic_expression -> byte_cod
      compile (Lit n) = PUSH n :: nil)
   /\
   (forall ae1 ae2 : arithmetic_expression,
-     compile (Plus ae1 ae2) = (compile ae1) ++ (compile ae2) ++ (ADD :: nil))
+     compile (Plus ae1 ae2) = (compile ae2) ++ (compile ae1) ++ (ADD :: nil))
   /\
   (forall ae1 ae2 : arithmetic_expression,
-     compile (Times ae1 ae2) = (compile ae1) ++ (compile ae2)++ (MUL :: nil)).
+     compile (Times ae1 ae2) = (compile ae2) ++ (compile ae1)++ (MUL :: nil))
+  /\
+  (forall ae1 ae2 : arithmetic_expression,
+     compile (Minus ae1 ae2) = (compile ae2) ++ (compile ae1) ++ (SUB :: nil)).
 
 (* Exercise 6:
    Define a compiler as a function
@@ -233,11 +292,197 @@ Definition specification_of_compile (compile : arithmetic_expression -> byte_cod
    and uses list concatenation, i.e., ++.
 *)
 
+Fixpoint compile_plusplus (ae : arithmetic_expression) : byte_code_program :=
+  match ae with
+    | Lit n => (PUSH n) :: nil
+    | Plus ae1 ae2 => (compile_plusplus ae2) ++ (compile_plusplus ae1) ++ (ADD :: nil)
+    | Times ae1 ae2 => (compile_plusplus ae2) ++ (compile_plusplus ae1) ++ (MUL :: nil)
+    | Minus ae1 ae2 => (compile_plusplus ae2) ++ (compile_plusplus ae1) ++ (SUB :: nil)
+  end.
+
+Lemma unfold_compile_plusplus_lit :
+  forall n : nat,
+    compile_plusplus (Lit n) = (PUSH n) :: nil.
+Proof.
+  unfold_tactic compile_plusplus.
+Qed.
+
+Lemma unfold_compile_plusplus_plus :
+  forall ae1 ae2 : arithmetic_expression,
+    compile_plusplus (Plus ae1 ae2) = (compile_plusplus ae2) ++ (compile_plusplus ae1) ++ (ADD :: nil).
+Proof.
+  unfold_tactic compile_plusplus.
+Qed.
+
+Lemma unfold_compile_plusplus_times :
+  forall ae1 ae2 : arithmetic_expression,
+    compile_plusplus (Times ae1 ae2) = (compile_plusplus ae2) ++ (compile_plusplus ae1) ++ (MUL :: nil).
+Proof.
+  unfold_tactic compile_plusplus.
+Qed.
+
+Lemma unfold_compile_plusplus_minus :
+  forall ae1 ae2 : arithmetic_expression,
+    compile_plusplus (Minus ae1 ae2) = (compile_plusplus ae2) ++ (compile_plusplus ae1) ++ (SUB :: nil).
+Proof.
+  unfold_tactic compile_plusplus.
+Qed.
+
+Theorem compile_plusplus_fits_the_specification_of_compile :
+  forall ae : arithmetic_expression,
+    specification_of_compile compile_plusplus.
+Proof.
+  unfold specification_of_compile.
+  split.
+    intro n.
+    apply (unfold_compile_plusplus_lit).
+    
+    split.
+      intros ae1 ae2.
+      apply (unfold_compile_plusplus_plus).
+
+      split.
+        intros ae1 ae2.
+        apply (unfold_compile_plusplus_times).
+
+        intros ae1 ae2.
+        apply (unfold_compile_plusplus_minus).
+Qed.
+
 (* Exercise 7:
    Write a compiler as a function with an accumulator
    that does not use ++ but :: instead,
    and prove it equivalent to the compiler of Exercise 6.
 *)
+
+Fixpoint compile_acc (ae : arithmetic_expression) (acc : byte_code_program) : byte_code_program :=
+  match ae with
+    | Lit n => (PUSH n) :: acc
+    | Plus ae1 ae2 => (compile_acc ae2 (compile_acc ae1 (ADD :: acc)))
+    | Times ae1 ae2 => (compile_acc ae2 (compile_acc ae1 (MUL :: acc)))
+    | Minus ae1 ae2 => (compile_acc ae2 (compile_acc ae1 (SUB :: acc)))
+  end.
+
+Compute(compile_acc (Plus (Lit 5) (Lit 3)) nil).
+
+Lemma unfold_compile_acc_lit :
+  forall (n : nat) (acc : byte_code_program),
+    compile_acc (Lit n) acc = (PUSH n) :: acc.
+Proof.
+  unfold_tactic compile_acc.
+Qed.
+
+Lemma unfold_compile_acc_plus :
+  forall (ae1 ae2 : arithmetic_expression) (acc : byte_code_program),
+    compile_acc (Plus ae1 ae2) acc = compile_acc ae2 (compile_acc ae1 (ADD :: acc)).
+Proof.
+  unfold_tactic compile_acc.
+Qed.
+
+Lemma unfold_compile_acc_times :
+  forall (ae1 ae2 : arithmetic_expression) (acc : byte_code_program),
+    compile_acc (Times ae1 ae2) acc = compile_acc ae2 (compile_acc ae1 (MUL :: acc)).
+Proof.
+  unfold_tactic compile_acc.
+Qed.
+
+Lemma unfold_compile_acc_minus :
+  forall (ae1 ae2 : arithmetic_expression) (acc : byte_code_program),
+    compile_acc (Minus ae1 ae2) acc = compile_acc ae2 (compile_acc ae1 (SUB :: acc)).
+Proof.
+  unfold_tactic compile_acc.
+Qed.
+
+
+
+Compute(execute_byte_code_program(compile_plusplus (Minus (Lit 5) (Lit 3))) nil).
+
+Compute(execute_byte_code_program(compile_plusplus (Minus (Lit 3) (Lit 5))) nil).
+
+Compute(execute_byte_code_program(compile_acc (Minus (Lit 5) (Lit 3)) nil) nil).
+
+Compute(execute_byte_code_program(compile_acc (Minus (Lit 3) (Lit 5)) nil) nil).
+
+
+
+(* EUREKA *)
+
+Lemma about_compile_acc :
+  forall (ae : arithmetic_expression) (acc bcp : byte_code_program),
+    (compile_acc ae acc) ++ bcp = compile_acc ae (acc ++ bcp).
+Proof.
+  intro ae.
+  induction ae as [ n | ae1 IHa1 ae2 IHa2 | ae1' IHa1' ae2' IHa2' | ae1'' IHa1'' ae2'' IHa2'' ].
+
+  intros acc bcp.
+  rewrite ->2 (unfold_compile_acc_lit).
+  Check(app_comm_cons).
+  rewrite <- (app_comm_cons).
+  reflexivity.
+
+  intros acc bcp.
+  rewrite ->2 (unfold_compile_acc_plus).
+  rewrite -> (app_comm_cons).
+  rewrite <- (IHa1 (ADD :: acc) bcp).
+  rewrite <- (IHa2). 
+  reflexivity.
+  
+  intros acc bcp.
+  rewrite ->2 (unfold_compile_acc_times).
+  rewrite -> (app_comm_cons).
+  rewrite <- (IHa1' (MUL :: acc) bcp).
+  rewrite <- (IHa2').
+  reflexivity.
+
+  intros acc bcp.
+  rewrite ->2 (unfold_compile_acc_minus).
+  rewrite -> (app_comm_cons).
+  rewrite <- (IHa1'' (SUB :: acc) bcp).
+  rewrite <- (IHa2'').
+  reflexivity.
+Qed.
+
+Lemma compile_plusplus_fits_compile_acc :
+  forall (ae : arithmetic_expression) (acc : byte_code_program),
+    compile_acc ae acc = (compile_plusplus ae) ++ acc.
+Proof.
+  intro ae.
+  induction ae as [ n | ae1 IHa1 ae2 IHa2 | ae1' IHa1' ae2' IHa2' | ae1'' IHa1'' ae2'' IHa2''].
+  intro acc.
+  rewrite -> (unfold_compile_acc_lit).
+  rewrite -> (unfold_compile_plusplus_lit).
+  unfold app.
+  reflexivity.
+
+  intro acc.
+  rewrite -> (unfold_compile_acc_plus).
+  rewrite -> (unfold_compile_plusplus_plus).
+  rewrite <- (IHa1).
+  rewrite <- (IHa2).
+  rewrite ->2 (about_compile_acc).
+  unfold app.
+  reflexivity.
+
+  intro acc.
+  rewrite -> (unfold_compile_acc_times).
+  rewrite -> (unfold_compile_plusplus_times).
+  rewrite <- (IHa1').
+  rewrite <- (IHa2').
+  rewrite ->2 (about_compile_acc).
+  unfold app.
+  reflexivity.
+
+  intro acc.
+  rewrite -> (unfold_compile_acc_minus).
+  rewrite -> (unfold_compile_plusplus_minus).
+  rewrite <- (IHa1'').
+  rewrite <- (IHa2'').
+  rewrite ->2 (about_compile_acc).
+  unfold app.
+  reflexivity.
+
+Qed.
+
 
 (* ********** *)
 
@@ -247,6 +492,49 @@ Definition specification_of_compile (compile : arithmetic_expression -> byte_cod
    over an empty data stack.
   INDUCTION ON THE AE
 *)
+
+
+
+Definition check_stack (stack : data_stack) : nat :=
+  match stack with
+    | x :: nil => x
+    | _ => 0
+  end.
+
+Check(specification_of_compile).
+Check(specification_of_interpret).
+
+
+
+Lemma executing_compile_is_the_same_as_interpreting :
+  forall (ae : arithmetic_expression),
+    interpreter ae = check_stack ( execute_byte_code_program (compile_acc ae nil) nil).
+Proof.
+  intro ae.
+  induction ae as [ a | ae1 IHa1 ae2 IHa2 | ae1' IHa1' ae2' IHa2' | ae1'' IHa1'' ae2'' IHa2''].
+
+  rewrite -> (unfold_interpreter_lit).
+  rewrite -> (unfold_compile_acc_lit).
+  rewrite -> (unfold_byte_code_program_ic).
+  rewrite -> (unfold_byte_code_program_bc).
+  unfold execute_byte_code_instruction.
+  unfold check_stack.
+  reflexivity.
+
+  rewrite -> (unfold_interpreter_plus).
+  rewrite -> (unfold_compile_acc_plus).
+
+  rewrite -> (IHa1).
+  rewrite -> (IHa2).
+  rewrite ->4 (compile_plusplus_fits_compile_acc).
+  rewrite <- (about_list_of_instructions).
+  SearchAbout(app).
+  rewrite -> (app_assoc).
+  rewrite -> (about_list_of_instructions).
+  rewrite <-3 (compile_plusplus_fits_compile_acc).
+
+  rewrite -> (unfold_byte_code_program_ic).
+
 
 (* ********** *)
 
